Added hook structure to the worlds.

Core/Worlds.v
@@ -18,7 +18,32 @@ Section WorldGetters.
 (* World is a dependent partial map of protocols *)
 
 Definition context := union_map Label protocol.
-Definition world := context.
+
+(* 
+The hooks are dependencies between:
+
+1. a hook's unique id
+2. a core protocol
+3. a client protocol
+4. a send-transition (represented by its tag) of a client protocol
+
+*)
+Definition hook_domain := [ordType of ((nat * Label) * (Label * nat))%type].
+
+(*
+
+A hook is a constraint from the local state wrt. core protocol (1st
+heap argument), relating the local state wrt. the client protocol (2ns
+heap argument), message to be sent, and the destination node id.
+
+*)
+Definition hook_type := heap -> heap -> seq nat -> nid -> Prop.
+
+Definition hooks := union_map hook_domain hook_type.
+Definition world := (context * hooks)%type.
+
+Definition getc (w: world) : context := fst w.
+Coercion getc : world >-> context.
 
 Variable w : world.
 
@@ -27,7 +52,7 @@ Variables (p : protocol).
 (* The function is, in fact, partially defined and returns Empty
    Protocol for a non-present label. *)
 Definition getProtocol i : protocol:=
-  match find i w with
+  match find i (getc w) with
   | Some p => p
   | None => EmptyProt i 
   end.
@@ -46,21 +71,29 @@ Section Core.
 
 (* The following definition ties together worlds and states *)
 
+Definition hooks_consistent (w : world) : Prop :=
+  let: (c, h) := w in
+  forall z lc ls t, ((z, lc), (ls, t)) \in dom h ->
+  (lc \in dom c) && (ls \in dom c).
+
 Definition Coh (w : world) : Pred state := fun s =>
-  [/\ valid w, valid s, dom w =i dom s &
+  let: c := fst w in
+  let: h := snd w in                                           
+  [/\ valid w, valid s, hooks_consistent w,
+      dom c =i dom s &
       forall l, coh (getProtocol w l) (getStatelet s l)].
 
 Lemma cohW w s : Coh w s -> valid w.
-Proof. by case. Qed.
+Proof. by case w=>[c h]; case. Qed.
 
 Lemma cohS w s : Coh w s -> valid s.
-Proof. by case. Qed.
+Proof. by case w=>[c h]; case. Qed.
 
-Lemma cohD w s : Coh w s -> dom w =i dom s.
-Proof. by case. Qed.
+Lemma cohD w s : Coh w s -> dom (getc w) =i dom s.
+Proof. by case w=>[c h]; case. Qed.
 
 Lemma coh_coh w s l : Coh w s -> coh (getProtocol w l) (getStatelet s l).
-Proof. by case. Qed.
+Proof. by case w=>[c h]; case. Qed.
 
 (* Now we need to establish a bunch of natural properties with respect
    to coherence of worlds and states. *)
@@ -68,53 +101,56 @@ Proof. by case. Qed.
 Lemma unit_coh w s :
   Coh w s -> w = Unit <-> s = Unit.
 Proof.
-case=>V V' E H; split=>Z; [subst w|subst s]; rewrite dom0 in E; last first.
-- by move/(dom0E V): E.
-have E': dom s =i pred0 by move=>z; move: (E z)=>->.
-by move/(dom0E V') : E'.
+case: (w)=>[c h].
+case=>V V' Hc E H; split.
+case=>Z1 Z2; subst c h; rewrite dom0 in E; last by rewrite (dom0E V').
+move=>Z; subst s; move/andP: V=>/=[V1 V2].
+have Z: c = Unit by apply: (dom0E V1); move=>z; rewrite E dom0.
+subst c; suff Z: (h = Unit) by subst h.
+simpl in Hc; clear E H V1 V'.
+apply: (dom0E V2); move=> x; case X: (x \in dom h)=>//.
+by move: x X=>[[z lc] [ls t]]/Hc/andP[]; rewrite !dom0. 
 Qed.
 
 Lemma Coh0 (w : world) (s : state) :
   w = Unit -> s = Unit -> Coh w s.
 Proof.
-move=>->->{w s}; split=>//=[|l]; first by rewrite !dom0.
-by rewrite /getProtocol /getStatelet !find0E. 
+move=>->->{w s}; split; rewrite ?dom0=>//=; last first.
+- by move=>l; rewrite /getProtocol /getStatelet !find0E.
+by move=>z lc ls t; rewrite dom0.  
 Qed.
-
-(* Lemma CohUnL (w1 w2 : world) (s1 s2 : state) : *)
-(*   Coh (w1 \+ w2) (s1 \+ s2) -> Coh w1 s1. *)
-(* Proof. *)
-(* case=>W V D H; split. *)
-(* - by move/validL: W. *)
-(* - by move/validL: V. *)
 
 Lemma CohUn (w1 w2 : world) (s1 s2 : state) :
   Coh w1 s1 -> Coh w2 s2 ->
   valid (w1 \+ w2) -> Coh (w1 \+ w2) (s1 \+ s2).
 Proof.
-move=>C1 C2 V.
-case: (C1)=>_ G1 J1 H1; case: (C2)=>_ G2 J2 H2.
+case: w1=>[c1 h1]; case: w2=>[c2 h2]; move=>C1 C2 V.
+case: (C1)=>_ G1 K1 J1 H1; case: (C2)=>_ G2 K2 J2 H2.
+case/andP: V=>V V'; simpl in V, V'.
 have X: valid (s1 \+ s2).
-- case: validUn=>//; [by rewrite G1|by rewrite G2|move=>l; rewrite -J1 -J2=>D1 D2].  
+- case: validUn=>//; [by rewrite G1|by rewrite G2|move=>l; rewrite -J1 -J2=>D1 D2].
   by case: validUn V=>//=V1 V2; move/(_ _ D1); rewrite D2.
-have Y: dom (w1 \+ w2) =i dom (s1 \+ s2).
-- move=>z; rewrite !domUn !inE/=; by rewrite V X/= J1 J2.  
-split=>// l; rewrite /getProtocol /getStatelet.
-case: (dom_find l (s1 \+ s2))=>[|v]Z.
-- move/find_none: (Z); rewrite -Y.
-  by case: dom_find=>//->_; rewrite Z.
-move/find_some: (Z)=>D; rewrite Z; rewrite -Y in D=> E.
-case: dom_find D=>// p Z' _ _; rewrite Z'.
-rewrite findUnL // in Z; rewrite findUnL // J1 in Z'.
-by case: ifP Z Z'=>_ F1 F2; [move: (H1 l)|move: (H2 l)];
-   rewrite /getProtocol /getStatelet F1 F2.
+have Y: dom (c1 \+ c2) =i dom (s1 \+ s2).
+- by move=>z; rewrite !domUn !inE/=;rewrite V X/= J1 J2.
+have Z1:  valid ((c1, h1) \+ (c2, h2)) by rewrite /valid/= V V'.
+split=>//[|l]; last first.
+- rewrite /getProtocol /getStatelet.
+  case: (dom_find l (s1 \+ s2))=>[|v]Z.
+  - by move/find_none: (Z); rewrite -Y; case: dom_find=>//->_; rewrite Z.
+  move/find_some: (Z)=>D; rewrite Z; rewrite -Y in D=> E.
+  case: dom_find D=>// p Z' _ _; rewrite Z'.
+  rewrite findUnL // in Z; rewrite findUnL // J1 in Z'.
+  by case: ifP Z Z'=>_ F1 F2; [move: (H1 l)|move: (H2 l)];
+     rewrite /getProtocol /getStatelet F1 F2.
+by move=>z lc ls t/=; rewrite domUn inE=>/andP[_]/orP[];[move/K1|move/K2];
+   move/andP=>[A1 A2]; rewrite !domUn !inE A1 A2 V -?(orbC true). 
 Qed.
 
 (* Coherence is trivially precise wrt. statelets *)
-Lemma coh_prec W: precise (Coh W).
+Lemma coh_prec w: precise (Coh w).
 Proof.
 move=>s1 s2 t1 t2 V E C1 C2.
-case: (C1)(C2)=>H1 G1 D1 _ [H2 G2 D2 _].
+case: (C1)(C2)=>H1 G1 K1 D1 _ [H2 G2 K2 D2 _].
 by apply: (@dom_prec _ _ _  s1 s2 t1 t2)=>//z; rewrite -D1 -D2.
 Qed.
 
@@ -132,8 +168,7 @@ Lemma locE' d n x y :
   valid (dstate d) ->
   getLocal n {| dstate := upd n x (dstate d);
                 dsoup := y |} = x.
-Proof.
-by move=>V; rewrite /getLocal findU eqxx/= V. Qed.
+Proof. by move=>V; rewrite /getLocal findU eqxx/= V. Qed.
 
 Lemma locU n n' x st s :
   n != n' ->
@@ -145,17 +180,17 @@ Proof.
   by rewrite /getLocal findU/= N.
 Qed.
 
+
 Section MakeWorld.
 
 Variable p : protocol.
 Notation l := (plab p).
 
-Definition mkWorld : world := l \\-> p.
+Definition mkWorld : world := (l \\-> p, Unit).
 
 Lemma prEq : (getProtocol mkWorld l) = p.
 Proof. by rewrite /getProtocol um_findPt. Qed.
-
-                            
+                          
 (*
 
 Here's an incomplete list of procedures and facts, which might be
